---
title: "Variance of a Binomial"
author: "Tony Nguyen"
date: "February 8, 2019"
output: 
  html_document: 
    toc: yes
    toc_float: yes
---

```{r setup, include=FALSE}
knitr::opts_chunk$set(echo = TRUE, message = FALSE)
```

# Introduction

We have learnt that the MGF for a binimial random variable is:

$$M_X(t) = (q+pe^t)^n $$

Where $X\sim Bin(n,p)$

# Tasks

Using the moment generating function above prove that 

$$\sigma^2 = npq$$

by answering the tasks below. 
Use $\LaTeX$ to construct the proof.

## Task 1

Start with 

$$
\begin{eqnarray}
E(X) &=& \left . \frac{d M_X(t)}{dt}\right |_{t=0}\\
\frac{dM_X(t)}{dt} &=& \frac{d}{dt}(q+pe^t)^n\\
u &=& q+pe^t, m=u^n\\
\frac{dM}{dt} &=& \frac{dM}{du}*\frac{du}{dt}\\
\frac{dM}{dt} &=& \frac{dM}{dt}
\end{eqnarray}
$$


## Task 2

Now find $E(X^2)$

$$
\begin{eqnarray}
E(X^2) &=& \left. \frac{d^2 M_X(t)}{dt^2}\right |_{t=0}\\
\frac{d^2 M_X(t)}{dt^2} &=& E(X(X-1))+E(X)\\
=n(n-1)p^2+np\\
=n^2p^2-np^2+np

\end{eqnarray}
$$

## Task 3

Find $\sigma^2$ Using the formula $\sigma^2 =E(X^2)-\mu^2$
Below I used substitution of E(X^2) and $\mu^2$.
$$
\begin{eqnarray}
\sigma^2 =E(X^2)-\mu^2 = \mu_1-(\mu_2)^2\\
\\
\\
\mu_1=\mu=\frac{d m_X(t)}{dt} |_{t=0}=n(pe^t+q)^(n-1)(pe^t) |_{t=0}\\
=n(pe^0+q)^(n-1)(pe^0)\\
\mu_1=\mu=n(p+q)^(n-1)p=n(1)^(n-1)p=np\\
\\
\\
\mu_2=\mu=\frac{d^2 m_X(t)}{dt^2} |_{t=0}=np\frac{d}{dt}[e^t(pe^t+q)^(n-1)] |_{t=0}\\
=np[e^t(n-1)(pe^t+q)^(n-2)pe^t+(pe^t+q)^(n-1)e^t] |_{t=0}\\
=np[(1)(n-1)(1)p+(1)(1)]=np[(n-1)p+1]\\
=np(np-p+1)=np(np+q)=n^2n^2+npq\\
\\
\\
\sigma^2 =n^2p^2+npq-(np)^2=npq\\
\end{eqnarray}
$$

